generic tactics for automatic proof of post condition

src/theory/tools/promising/strongPostCondLib.sml
@@ -7,7 +7,8 @@ struct
 
 open HolKernel Parse boolLib bossLib;
 open bir_programTheory bir_promisingTheory
-     bir_programLib bir_promising_wfTheory;
+     bir_programLib bir_promising_wfTheory
+     promising_thmsTheory ;
 
 Definition bst_pc_tuple_def:
   bst_pc_tuple x = (x.bpc_label,x.bpc_index)
@@ -58,6 +59,14 @@ map fst $ TypeBase.fields_of ``:bir_state_t``
 fun list_dest f tm =
   let val (x,y) = f tm in list_dest f x @ [y] end
   handle HOL_ERR _ => [tm];
+
+(* rewrite term with some simpset equalities and resort/deduplicate conjuncts *)
+fun simplify_term x =
+  REFL x
+  (* ++ boolSimps.DNF_ss *)
+  |> CONV_RULE $ RHS_CONV $ SIMP_CONV (srw_ss()) [AC CONJ_ASSOC CONJ_COMM,AND_CLAUSES,GSYM lock_addr_def,GSYM lock_addr_val_def]
+  |> rand o concl
+
 
 (*
 any property is maintained by jumps
@@ -176,6 +185,90 @@ fun bir_stmts_progs_thm prog =
   EVAL $ mk_icomb(``bir_stmts_of_progs``,prog)
   |> CONV_RULE $ RHS_CONV $ SIMP_CONV (srw_ss() ++ boolSimps.DNF_ss) [listTheory.MAP_APPEND,bir_typing_progTheory.bir_stmts_of_block_def]
 
+fun bir_stmts_term prog =
+  bir_stmts_progs_thm prog
+  |> concl |> rand
+  |> listSyntax.dest_list |> fst
+  |> map pairSyntax.dest_pair
+  handle HOL_ERR _ => raise ERR "function" "cannot destruct hol list of labels and stmts"
+
+(*
+list of collected constraints on registers
+find the known registers from
+map fst $ Redblackmap.listItems constr
+that are part of the jump constraint cjmp_constr
+*)
+
+(* jump stmt to constraints
+arguments
+  stmt          current statement
+  regs          list of register names (that may occur as dependents in jmp constraint)
+  cjmp_constr   map: address to constr
+                where the dependents are from regs list
+*)
+(*
+
+val cjmp_constr = Redblackmap.mkDict Term.compare : (term, constr) Redblackmap.dict
+val jmp_stmt =
+   ``BStmt_CJmp
+       (BExp_UnaryExp BIExp_Not
+          (BExp_BinPred BIExp_Equal (BExp_Den (BVar "x5" (BType_Imm Bit64)))
+             (BExp_Const (Imm64 0w))))
+       (BLE_Label (BL_Address (Imm64 lock_entry)))
+       (BLE_Label (BL_Address (Imm64 (lock_entry + 8w))))``
+val regs = [``BVar "x5" (BType_Imm Bit64)``];
+Redblackmap.listItems $ #2 $ jmp_stmt_to_constr jmp_stmt regs cjmp_constr
+
+*)
+
+fun jmp_stmt_to_constr jmp_stmt regs cjmp_constr =
+  case term_to_string_args jmp_stmt of
+    ("BStmt_CJmp", cond::lbl1::lbl2::[]) =>
+      let
+        (* TODO extract dependencies of regs from cond expression, e.g. by
+           evaluation, extracting all the variables *)
+        val deps = []
+        val cjmp_constr1 =
+          Redblackmap.insert(cjmp_constr, lbl2, { dependents = deps, constraint = cond })
+        val cond_neg = mk_icomb(``BExp_UnaryExp BIExp_Not``, cond)
+        val cjmp_constr2 =
+          Redblackmap.insert(cjmp_constr1, lbl1, { dependents = deps, constraint =  cond_neg})
+      in ([lbl1,lbl2],cjmp_constr2,true) end
+  | ("BStmt_Jmp", lbl::[]) => ([lbl],cjmp_constr,false)
+  | _ => ([],cjmp_constr,false) (* ignore other final stmts *)
+
+
+(* transforms a path and jump constraints into a conjunct
+   cjmp_path     list of jump target addresses that were jumped on this path
+   cjmp_constr   map of jump addresses to constraints
+ *)
+(*
+
+val cjmp_path = [``BLE_Label (BL_Address (Imm64 (lock_entry + 8w)))``,``BLE_Label (BL_Address (Imm64 lock_entry))``]
+val cjmp_constr = Redblackmap.mkDict Term.compare : (term, constr) Redblackmap.dict
+val jmp_stmt =
+   ``BStmt_CJmp
+       (BExp_UnaryExp BIExp_Not
+          (BExp_BinPred BIExp_Equal (BExp_Den (BVar "x5" (BType_Imm Bit64)))
+             (BExp_Const (Imm64 0w))))
+       (BLE_Label (BL_Address (Imm64 lock_entry)))
+       (BLE_Label (BL_Address (Imm64 (lock_entry + 8w))))``
+val regs = [``BVar "x5" (BType_Imm Bit64)``];
+val cjmp_constr = #2 $ jmp_stmt_to_constr jmp_stmt regs cjmp_constr
+
+Redblackmap.listItems cjmp_constr
+jmp_constr_to_term cjmp_constr path
+
+*)
+
+fun jmp_constr_to_term (cjmp_constr : (term, constr) Redblackmap.dict) (cjmp_path : term list) =
+    simplify_term $ foldl (fn (x,e) =>
+      let val v_opt = Redblackmap.peek(cjmp_constr,x)
+          val v_opt = Option.map #constraint v_opt
+          val v_opt = Option.map (fn v => bir_eval_exp_val v ``Imm1 1w``) v_opt
+      in if isSome v_opt then mk_conj(e, (valOf v_opt)) else e end
+    ) ``T`` cjmp_path
+
 (*
 
 arguments: jump_head
@@ -224,13 +317,6 @@ end
 fun is_term_true tm = is_eq_tm ``T`` tm
 fun is_term_false tm = is_eq_tm ``F`` tm
 
-(* rewrite term with some simpset equalities and resort/deduplicate conjuncts *)
-fun simplify_term x =
-  REFL x
-  (* ++ boolSimps.DNF_ss *)
-  |> CONV_RULE $ RHS_CONV $ SIMP_CONV (srw_ss()) [AC CONJ_ASSOC CONJ_COMM,AND_CLAUSES,GSYM lock_addr_def]
-  |> rand o concl
-
 (* returns conjunct of lbl_var equals addr and index_var equals index:num *)
 fun addr_label_cj_index addr index =
 let
@@ -252,6 +338,10 @@ in
     if null cjmp_constr then term else mk_conj(term,list_mk_conj $ map #constraint (cjmp_constr :constr list))
   )
 end
+
+(* print contstraints
+Redblackmap.listItems constr
+*)
 
 (* filter path conditions if dependency has changed *)
 fun filter_cjmp_constr cjmp_constr addrs =
@@ -280,6 +370,9 @@ end
 fun bir_eval_exp_den_imm variable value =
 ``bir_eval_exp (BExp_Den ^variable) s.bst_environ = SOME $ BVal_Imm ^value``
 
+fun bir_eval_exp_val tm value =
+``bir_eval_exp (^tm) s.bst_environ = SOME $ BVal_Imm ^value``
+
 (* updates tuple (mem,reg) according to stmt at pc where
  *   stmt is a statement
  *   pc is the current program counter
@@ -293,36 +386,43 @@ BMCStmt_Load:
 val var::exp::opt::acq::rel::_ = snd $ term_to_string_args stmt
 BMCStmt_Store:
 val succ_reg::address::value::xcl::acq::rel::_ = snd $ term_to_string_args stmt
+Redblackmap.listItems $ #1 $ update_constr stmt constr cjmp_constr
 *)
+
 fun update_constr stmt constr cjmp_constr =
-(* match against statement type and respective arguments *)
 case term_to_string_args stmt of
   ("BMCStmt_Load",   var::exp::opt::acq::rel::_) =>
   (*
-    val var::exp::opt::acq::rel::_ = tl stmt_args
+    val var::exp::_ = #2 $ term_to_string_args stmt
   *)
     (* not exhaustive *)
     (case term_to_string_args exp of
       ("BExp_Const", cexp_val::_) =>
+(*
+val ("BExp_Const",cexp_val::_) = term_to_string_args exp
+ *)
         (Redblackmap.insert(constr, Reg var,
             (* TODO set dependencies to parts of cexp_val for non-constants *)
             { dependents = [],
-            constraint = bir_eval_exp_den_imm var cexp_val
-              (* ``bir_eval_exp (BExp_Den ^var) s.bst_environ = SOME $ BVal_Imm $ ^cexp_val`` *)
-              (* keep path constraints for unchanged locations *)
+              constraint =
+              ``?v t. bir_read_reg (bir_var_name ^var) s.bst_environ v
+              /\ mem_read M (BVal_Imm ^cexp_val) t = SOME $ BVal_Imm $ Imm64 v``
+              (* read from address cexp_val into register var *)
             }
           ),
           filter_cjmp_constr cjmp_constr [var])
 (*
 val ("BExp_Den",var'::_) = term_to_string_args exp
  *)
-    | ("BExp_Den",var'::_) =>
+    | _ => (constr,cjmp_constr)
+    (*
+    ("BExp_Den",var'::_) =>
       (constr,
           { dependents = [var, var'],
             constraint =
               ``bir_eval_exp (BExp_BinPred BIExp_Equal (BExp_Den ^var') (BExp_Den ^var)) s.bst_environ = SOME $ BVal_Imm $ Imm1 1w``
           }::cjmp_constr)
-    )
+    *))
 | ("BMCStmt_Store",  succ_reg::address::value::xcl::acq::rel::_)
   =>
     let
@@ -334,20 +434,38 @@ val ("BExp_Den",var'::_) = term_to_string_args exp
           (* semantics: may fail if xcl *)
           if is_term_true xcl then
           ``
-            bir_eval_exp (BExp_Den ^succ_reg) s.bst_environ = SOME $ BVal_Imm v_succ
+            (?v. bir_eval_exp (BExp_Den ^succ_reg) s.bst_environ = SOME $ BVal_Imm $ Imm64 v)
+            /\ (bir_eval_exp (BExp_Den ^succ_reg) s.bst_environ = SOME $ BVal_Imm v_succ
             ==>
               ?val. mem_read M ^address' (s.bst_coh ^address') = SOME $ val
-              /\ bir_eval_exp ^value s.bst_environ = SOME val
+              /\ bir_eval_exp ^value s.bst_environ = SOME val)
           ``
           else
           ``
-            ?val. mem_read M ^address' (s.bst_coh ^address') = SOME $ val
+            (?v. bir_eval_exp (BExp_Den ^succ_reg) s.bst_environ = SOME $ BVal_Imm $ Imm64 v)
+            /\ ?val. mem_read M ^address' (s.bst_coh ^address') = SOME $ val
             /\ bir_eval_exp ^value s.bst_environ = SOME val
           ``,
         (* check if  *)
         dependents = [address',succ_reg]
       }), filter_cjmp_constr cjmp_constr [address',succ_reg])
     end
+| ("BMCStmt_Assign", var::exp::_) =>
+    (case term_to_string_args exp of
+      (* TODO non-exhaustive *)
+      ("BExp_Const", cexp_val::_) =>
+(*
+val ("BExp_Const",cexp_val::_) = term_to_string_args exp
+*)
+        (Redblackmap.insert(constr, Reg var,
+            (* TODO set dependencies to parts of cexp_val for non-constants *)
+            { dependents = [],
+              constraint = bir_eval_exp_den_imm var cexp_val
+              (* keep path constraints for unchanged locations *)
+            }
+          ),
+          filter_cjmp_constr cjmp_constr [var])
+    )
 (*
 | ("BMCStmt_Amo",    succ_reg::address::value::acq::rel::_) => constr
 | ("BMCStmt_Assign", var::exp::_) => constr
@@ -420,11 +538,11 @@ let
     (case (has_visited target_t, has_visited target_f) of
       (true,false) =>
           (target_f,{ constraint =
-              ``bir_eval_exp ^cond (^s).bst_environ = SOME $ BVal_Imm $ Imm1 1w``
+              ``bir_eval_exp ^cond (^s).bst_environ = SOME $ BVal_Imm $ Imm1 0w``
           ,  dependents = cond_locs})
     | (false,true) =>
           (target_t,{ constraint =
-            ``bir_eval_exp ^cond (^s).bst_environ = SOME $ BVal_Imm $ Imm1 0w``
+            ``bir_eval_exp ^cond (^s).bst_environ = SOME $ BVal_Imm $ Imm1 1w``
           ,  dependents = cond_locs})
     )
     handle _ =>
@@ -438,6 +556,11 @@ handle _ =>
 
 fun get_jmp_target jmp_stmt =
   hd $ unpack "BLE_Label" $ hd $ unpack "BStmt_Jmp" jmp_stmt
+  handle _ =>
+    raise ERR "get_jmp_target" "unhandled jump target"
+
+fun get_cjmp_targets jmp_stmt =
+  map (hd o unpack "BLE_Label") (tl $ unpack "BStmt_CJmp" jmp_stmt)
   handle _ =>
     raise ERR "get_jmp_target" "unhandled jump target"
 
@@ -521,8 +644,9 @@ case fst $ term_to_string_args jmp_stmt of
 val constr = #constr s
 val cjmp_constr = #cjmp_constr s
 val visited_pcs = #visited_pcs s
+Redblackmap.listItems constr
  *)
-fun block_constr constr cjmp_constr addr stmts jmp_stmt visited_pcs (lc : lc) =
+fun block_constr constr cjmp_constr addr stmts jmp_stmt visited_pcs cjmp_path (lc : lc) =
 let
   (* constr and post condition *)
   val (constr,cjmp_constr,block_term,lc) =
@@ -530,39 +654,51 @@ let
       (fn ((index,stmt), (constr,cjmp_constr,term,lc)) =>
         let
 (*
-val stmt = hd stmts
-val index = 0
+val (index,stmt) =  (fn n => (n,List.nth(stmts,n))) 0
 val cjmp_constr = []
 val term = ``T``
 *)
-          val (constr,cjmp_constr) = update_constr stmt constr cjmp_constr
+          (* constraint at current pc is collection of previous constraints *)
           val term' =
             constrs_to_term (addr,index) constr cjmp_constr
+          val (constr,cjmp_constr) = update_constr stmt constr cjmp_constr
           (* linearisation constraint only needs to remember index and label of
              change of  *)
           val lc = lin_constr lc (addr,index,stmt)
         in
 (*
-          val term = mk_conj(term,term')
+          val term = simplify_term $ mk_conj(term,term')
  *)
-          (constr,cjmp_constr,mk_conj(term,term'),lc)
+          (constr,cjmp_constr,simplify_term $ mk_conj(term,term'),lc)
         end
       )
       (constr,cjmp_constr,``T``,lc)
       (mapi pair stmts)
+  val jmp_term = constrs_to_term (addr,length stmts) constr cjmp_constr
+  val block_post_cond = simplify_term $ mk_conj(block_term, jmp_term)
   (* case split on the jump kind *)
   (* TODO should branch if neither addr has been visited before *)
+(*
+  val (targets,cjmp_constr,is_cjmp) = jmp_stmt_to_constr jmp_stmt regs cjmp_constr
+*)
   val (target,cjmp_constr) =
     case fst $ term_to_string_args jmp_stmt of
       "BStmt_CJmp" => assemble_cjmp_constr (constr,cjmp_constr,visited_pcs) jmp_stmt
     | "BStmt_Jmp" => (get_jmp_target jmp_stmt,cjmp_constr)
     | _ => (addr,cjmp_constr) (* ignore other final stmts *)
+  (* TODO extract addresses from cjmp_constr and add to constr *)
   val lc = update_lc_jmp (addr,length stmts,jmp_stmt) lc
+(* TODO choose proper address (branch!) *)
+(*
+   val target =
+    if is_cjmp
+      then hd $ List.filter (fn x => not (List.member x visited_pcs)) targets
+      else target
+   val cjmp_path = if is_cjmp cjmp_path then target::cjmp_path else cjmp_path
+*)
   val visited_pcs = visited_pcs@[addr]
-  val jmp_term = constrs_to_term (target,length stmts) constr cjmp_constr
-  val block_post_cond = simplify_term $ mk_conj(block_term, jmp_term)
 in
-  (target, visited_pcs, block_post_cond, constr, cjmp_constr, lc)
+  (target, visited_pcs, block_post_cond, constr, cjmp_constr, cjmp_path, lc)
 end
 
 (*
@@ -582,16 +718,10 @@ val prog = ``BirProgram $ dequeue (BExp_Const $ Imm64 42w) (BExp_Const $ Imm64 4
 *)
 
 val prog = ``BirProgram $ unlock lock_addr unlock_entry``
-val prog = ``BirProgram $ lock lock_addr lock_entry jump_after``
+val prog = ``BirProgram (lock lock_addr lock_entry jump_after : (bmc_stmt_basic_t, mem_msg_t list # num list) bir_generic_block_t list)``
 
 (* (bir_label_t # option) list *)
-val label_stmts_thm = bir_stmts_progs_thm prog
-val labels_stmts_list =
-  SPEC_ALL label_stmts_thm |> concl |> rand
-  |> listSyntax.dest_list |> fst
-  |> map pairSyntax.dest_pair
-  handle HOL_ERR _ => raise ERR "function" "cannot destruct hol list of labels and stmts"
-
+val labels_stmts_list = bir_stmts_term prog
 (* get block statements at address *)
 (* label # stmt term list # jmp *)
 val addresses_stmts =
@@ -613,8 +743,6 @@ val stmt = List.nth (stmts, 0)
 val len = length stmts
 *)
 
-(* assumption that the control flow is linear for this code *)
-
 (*
 val term = ``T``
 val stmt = hd stmts
@@ -625,7 +753,8 @@ val init_state = {
     constr = Redblackmap.mkDict kind_cmp : (kind, constr) Redblackmap.dict,
     cjmp_constr = [] : constr list,
     post_conds = ``T``,
-    visited_pcs = [] : term list
+    visited_pcs = [] : term list,
+    cjmp_path = [] : term list (* path of jumped-to jump targets *)
 };
 val s = init_state;
 (* matching the type lc *)
@@ -643,21 +772,21 @@ val lc = {
    the current equivalence class of linearisation points gets swapped after completing the block that contains a successful store to lin_addr
 *)
 
-val ({constr,cjmp_constr,post_conds,visited_pcs},lc) =
+val ({constr,cjmp_constr,post_conds,visited_pcs,cjmp_path},lc) =
   List.foldl (fn ((addr,stmts,jmp_stmt),(s,lc)) =>
     let
       (* assume that next addr == target *)
 (*
-      val (addr,stmts,jmp_stmt) = List.nth (addresses_stmts,0);
+      val (addr,stmts,jmp_stmt) = List.nth (addresses_stmts,3);
       val (target, visited_pcs, block_post_cond, constr, cjmp_constr, lc) =
         block_constr (#constr s) (#cjmp_constr s) addr stmts jmp_stmt (#visited_pcs s) lc
       val s =
       {constr=constr,cjmp_constr=cjmp_constr,post_conds=simplify_term $ mk_conj(#post_conds s,block_post_cond),visited_pcs=visited_pcs}
 *)
-      val (target, visited_pcs, block_post_cond, constr, cjmp_constr, lc) =
-        block_constr (#constr s) (#cjmp_constr s) addr stmts jmp_stmt (#visited_pcs s) lc
+      val (target, visited_pcs, block_post_cond, constr, cjmp_constr, cjmp_path, lc) =
+        block_constr (#constr s) (#cjmp_constr s) addr stmts jmp_stmt (#visited_pcs s) (#cjmp_path s) lc
     in
-      ({constr=constr,cjmp_constr=cjmp_constr,post_conds=simplify_term $ mk_conj(#post_conds s,block_post_cond),visited_pcs=visited_pcs},lc)
+      ({constr=constr,cjmp_constr=cjmp_constr,post_conds=simplify_term $ mk_conj(#post_conds s,block_post_cond),visited_pcs=visited_pcs,cjmp_path=cjmp_path},lc)
     end
   )
   (init_state,lc)
@@ -672,11 +801,416 @@ val lin_term =
     )
     (mapi pair ((#old lc)@[#current lc]))
 
+(*
+
 ^lin_term
+
+post_conds
+lock_def
+
+*)
 
 (*
 $HOLDIR/src/portableML/Redblackmap.sig
 wordsSyntax.mk_wordii (255, 8) (* 8w:word4 *)
 *)
+
+(* constraints particular for this program *)
+(* has to quantify all arguments to lock_def *)
+Definition prog_individual_constraints_def:
+  prog_individual_constraints lock_entry jump_after
+  = ?x. jump_after = BL_Address (Imm64 x)
+  /\ ~(MEM jump_after $ bir_labels_of_program ^prog)
+End
+
+(* bir_get_current_statement equalities *)
+val prog_bgcs = save_thm("prog_bgcs", bgcs_bmc_prog_thms prog);
+
+(* trivial: no external statements *)
+val prog_wf_ext = store_thm("prog_wf_ext",
+  ``wf_ext ^prog cid c M``,
+  fs[prog_bgcs,wf_ext_def,wf_ext_p_def]);
+
+val prog_blop = save_thm("prog_blop", blop_prog_labels_thm prog)
+
+Theorem prog_individual_constraints_eq =
+  REWRITE_RULE[prog_blop] prog_individual_constraints_def
+  |> CONV_RULE $ SIMP_CONV (srw_ss() ++ boolSimps.DNF_ss) []
+
+(* for parameterised labels we assume disjointness *)
+val prog_blop_ALL_DISTINCT_tm =
+  ``ALL_DISTINCT $ bir_labels_of_program ^prog``
+ (*``ALL_DISTINCT ^(prog_blop |> concl |> rator |> rand)``*)
+
+val prog_blop_ALL_DISTINCT = EVAL prog_blop_ALL_DISTINCT_tm
+  |> CONV_RULE $ RHS_CONV $ SIMP_CONV (srw_ss() ++ boolSimps.DNF_ss) [AC CONJ_ASSOC CONJ_COMM,wordsTheory.dimword_64]
+
+val post_cond_def = Define `
+  post_cond M s lock_entry =
+    !lbl index. bst_pc_tuple s.bst_pc = (BL_Address $ Imm64 lbl, index)
+      ==> ^post_conds
+  `
+
+(* assumption:
+- distinct addresses is necessary due to parametrised addresses:
+  ALL_DISTINCT $ bir_labels_of_program prog
+- memory only holds values of certain fixed type: wf_mem_vals
+- wellformed labels for jump outside (disjointness)
+  jump outside of the program labels which are disjoint 
+  prog_individual_constraints
+
+
+TODO prove invariant wf_mem_vals
+can we generally prove the invariant for
+  certifying trace P ==> wf_mem_val P /\ wf_mem_loc P
+
+*)
+
+(* generic tactis for 12 theorems, see clstep_bgcs_cases *)
+
+val clstep_post_cond_inv_tac =
+  rpt strip_tac
+  >> imp_res_tac clstep_bgcs_imp
+  >> drule_then assume_tac bir_get_current_statement_SOME_MEM
+  >> drule_at (Pat `clstep`) clstep_preserves_wf
+  >> disch_then $ drule_at_then Any assume_tac
+  >> fs[prog_wf_ext]
+  >> imp_res_tac clstep_bgcs_cases
+  >> gvs[]
+  >> gs[post_cond_def,clstep_cases,bst_pc_tuple_def,bir_pc_next_def,bmc_exec_general_stmt_exists,bir_state_read_view_updates_def]
+
+Theorem clstep_post_cond_inv_BMCStmt_Load:
+  clstep (^prog) cid c M prom c'
+  /\ post_cond M c lock_entry
+  /\ well_formed cid M c
+  /\ wf_mem_vals M
+  /\ prog_individual_constraints lock_entry jump_after
+  /\ ^prog_blop_ALL_DISTINCT_tm
+  /\ bir_get_current_statement ^prog c.bst_pc = SOME $ BSGen $ BStmtB $ BMCStmt_Load var a_e opt_cast xcl acq rel
+  ==> post_cond M c' lock_entry
+Proof
+  clstep_post_cond_inv_tac
+  (* BMCStmt_Load specific *)
+  >> gvs[prog_bgcs,AND_IMP_INTRO,IMP_CONJ_THM,FORALL_AND_THM,prog_blop_ALL_DISTINCT]
+  (* use distinctness of labels to solve all other issues *)
+  >> qpat_assum `_ = c_bst_pc.bpc_label` $ assume_tac o GSYM
+  >> fs[bir_read_reg_prime,lock_addr_def,lock_addr_val_def]
+  >> fs[bir_envTheory.bir_var_name_def,bir_envTheory.bir_var_type_def]
+  >> drule_all_then strip_assume_tac wf_mem_vals_mem_read
+  >> fs[bir_eval_exp_view_def,cj 1 bir_expTheory.bir_eval_exp_def]
+  >> goal_assum $ drule_at $ Pat `mem_read`
+  >> drule $ GSYM bir_read_reg_env_update_cast64
+  >> fs[]
+QED
+
+Theorem clstep_post_cond_inv_BMCStmt_Store_fail:
+  clstep (^prog) cid c M prom c'
+  /\ post_cond M c lock_entry
+  /\ well_formed cid M c
+  /\ wf_mem_vals M
+  /\ prog_individual_constraints lock_entry jump_after
+  /\ ^prog_blop_ALL_DISTINCT_tm
+  /\ bir_get_current_statement ^prog c.bst_pc = SOME $ BSGen $ BStmtB $ BMCStmt_Store var_succ a_e v_e xcl acq rel
+  /\ prom = [] /\ xcl
+  ==> post_cond M c' lock_entry
+Proof
+  clstep_post_cond_inv_tac
+  (* BMCStmt_Store *)
+  >> fs[prog_blop_ALL_DISTINCT]
+  >> gvs[prog_bgcs]
+  >> fs[AND_IMP_INTRO,IMP_CONJ_THM,FORALL_AND_THM]
+  >> qpat_assum `_ = c_bst_pc.bpc_label` $ assume_tac o GSYM
+  >> fs[wordsTheory.dimword_64]
+  >> gs[xclfail_update_env_SOME,bir_eval_exp_BExp_Den_update_eq']
+  >> fs[bir_eval_exp_BExp_Den_update_eq,v_fail_def,v_succ_def]
+QED
+
+Theorem clstep_post_cond_inv_BMCStmt_Store:
+  clstep (^prog) cid c M prom c'
+  /\ post_cond M c lock_entry
+  /\ well_formed cid M c
+  /\ wf_mem_vals M
+  /\ prog_individual_constraints lock_entry jump_after
+  /\ ^prog_blop_ALL_DISTINCT_tm
+  /\ bir_get_current_statement ^prog c.bst_pc = SOME $ BSGen $ BStmtB $ BMCStmt_Store var_succ a_e v_e xcl acq rel
+  /\ ~(NULL prom)
+  ==> post_cond M c' lock_entry
+Proof
+  clstep_post_cond_inv_tac
+  (* BMCStmt_Store *)
+  >> fs[prog_blop_ALL_DISTINCT]
+  >> gvs[prog_bgcs]
+  >> fs[AND_IMP_INTRO,IMP_CONJ_THM,FORALL_AND_THM]
+  >> qpat_assum `_ = c_bst_pc.bpc_label` $ assume_tac o GSYM
+  >> fs[wordsTheory.dimword_64,bir_state_fulful_view_updates_def]
+  >> gs[fulfil_update_env_BVar_eq,bir_eval_exp_BExp_Den_update_eq']
+  >> fs[bir_eval_exp_BExp_Den_update_eq,v_succ_def]
+  >> fs[bir_eval_exp_view_def,cj 1 bir_expTheory.bir_eval_exp_def,lock_addr_val_def,combinTheory.APPLY_UPDATE_THM,mem_read_def]
+QED
+
+Theorem clstep_post_cond_inv_BMCStmt_Amo:
+  clstep (^prog) cid c M prom c'
+  /\ post_cond M c lock_entry
+  /\ well_formed cid M c
+  /\ wf_mem_vals M
+  /\ prog_individual_constraints lock_entry jump_after
+  /\ ^prog_blop_ALL_DISTINCT_tm
+  /\ bir_get_current_statement ^prog c.bst_pc = SOME $ BSGen $ BStmtB $ BMCStmt_Amo var a_e v_e acq rel
+  ==> post_cond M c' lock_entry
+Proof
+  clstep_post_cond_inv_tac
+  (* BMCStmt_Amo *)
+  (* TODO generalise with same reasoning as BMCStmt_Store *)
+  >> gvs[prog_bgcs]
+QED
+
+Theorem clstep_post_cond_inv_BMCStmt_Fence:
+  clstep (^prog) cid c M prom c'
+  /\ post_cond M c lock_entry
+  /\ well_formed cid M c
+  /\ wf_mem_vals M
+  /\ prog_individual_constraints lock_entry jump_after
+  /\ ^prog_blop_ALL_DISTINCT_tm
+  /\ bir_get_current_statement ^prog c.bst_pc = SOME $ BSGen $ BStmtB $ BMCStmt_Fence K1 K2
+  ==> post_cond M c' lock_entry
+Proof
+  clstep_post_cond_inv_tac
+  (* BMCStmt_Fence *)
+  (* TODO implement for program *)
+  >> gvs[prog_bgcs]
+QED
+
+Theorem clstep_post_cond_inv_BMCStmt_CJmp:
+  clstep (^prog) cid c M prom c'
+  /\ post_cond M c lock_entry
+  /\ well_formed cid M c
+  /\ wf_mem_vals M
+  /\ prog_individual_constraints lock_entry jump_after
+  /\ ^prog_blop_ALL_DISTINCT_tm
+  /\ bir_get_current_statement ^prog c.bst_pc = SOME $ BSGen $ BStmtE $ BStmt_CJmp cond_e lbl1 lbl2
+  ==> post_cond M c' lock_entry
+Proof
+  clstep_post_cond_inv_tac
+  (* BStmt_CJmp *)
+  >> fs[prog_blop_ALL_DISTINCT]
+  (* possible branching here due to several jumps *)
+  >> gvs[prog_bgcs]
+  >> fs[AND_IMP_INTRO,IMP_CONJ_THM,FORALL_AND_THM]
+  >> qpat_assum `_ = c_bst_pc.bpc_label` $ assume_tac o GSYM
+  >> fs[wordsTheory.dimword_64,bir_exec_stmt_cjmp_mc_invar]
+  >> fs[bir_exec_stmt_cjmp_def,bir_eval_exp_view_def,Once bir_eval_exp_SOME']
+  >> gvs[v_succ_def,GSYM bir_read_reg_def,bir_read_reg_bir_env_read,bir_envTheory.bir_var_name_def]
+  >> drule_then (gvs o single) bir_eval_exp_BExp_UnaryExp'
+  >> fs[bir_valuesTheory.bir_dest_bool_val_def]
+  >> qmatch_goalsub_abbrev_tac `COND cond _ _`
+  >> Cases_on `cond`
+  >> fs[bir_exec_stmt_jmp_def,bir_eval_label_exp_def,bir_exec_stmt_jmp_to_label_mc_invar]
+  >> fs[bir_exec_stmt_jmp_to_label_def,prog_blop,bir_block_pc_def]
+  >> fs[wordsTheory.dimword_64,prog_individual_constraints_eq]
+  >> fs[COND_RAND,COND_RATOR]
+  >> drule_then (fs o single) bir_eval_exp_BExp_UnaryExp
+  >> goal_assum drule_all
+  >> fs[]
+QED
+
+Theorem clstep_post_cond_inv_BMCStmt_Assign:
+  clstep (^prog) cid c M prom c'
+  /\ post_cond M c lock_entry
+  /\ well_formed cid M c
+  /\ wf_mem_vals M
+  /\ prog_individual_constraints lock_entry jump_after
+  /\ ^prog_blop_ALL_DISTINCT_tm
+  /\ bir_get_current_statement ^prog c.bst_pc = SOME $ BSGen $ BStmtB $ BMCStmt_Assign var e
+  ==> post_cond M c' lock_entry
+Proof
+  clstep_post_cond_inv_tac
+  (* BMCStmt_Assign *)
+  >> gvs[prog_bgcs,AND_IMP_INTRO,IMP_CONJ_THM,FORALL_AND_THM,prog_blop_ALL_DISTINCT]
+  (* use distinctness of labels to solve all other issues *)
+  >> qpat_assum `_ = c_bst_pc.bpc_label` $ assume_tac o GSYM
+  >> fs[bir_envTheory.bir_var_name_def,bir_envTheory.bir_var_type_def,bir_eval_exp_view_def,cj 1 bir_expTheory.bir_eval_exp_def,wordsTheory.dimword_64,bir_read_reg_bir_env_read,GSYM bir_read_reg_def]
+  >> drule $ GSYM bir_read_reg_env_update_cast64
+  >> fs[]
+QED
+
+Theorem clstep_post_cond_inv_BMCStmt_Assert:
+  clstep (^prog) cid c M prom c'
+  /\ post_cond M c lock_entry
+  /\ well_formed cid M c
+  /\ wf_mem_vals M
+  /\ prog_individual_constraints lock_entry jump_after
+  /\ ^prog_blop_ALL_DISTINCT_tm
+  /\ bir_get_current_statement ^prog c.bst_pc = SOME $ BSGen $ BStmtB $ BMCStmt_Assert e
+  ==> post_cond M c' lock_entry
+Proof
+  clstep_post_cond_inv_tac
+  (* BMCStmt_Assert *)
+  >> gvs[prog_bgcs,AND_IMP_INTRO,IMP_CONJ_THM,FORALL_AND_THM,prog_blop_ALL_DISTINCT]
+  >> qpat_assum `_ = c_bst_pc.bpc_label` $ assume_tac o GSYM
+  >> fs[]
+QED
+
+Theorem clstep_post_cond_inv_BMCStmt_Assume:
+  clstep (^prog) cid c M prom c'
+  /\ post_cond M c lock_entry
+  /\ well_formed cid M c
+  /\ wf_mem_vals M
+  /\ prog_individual_constraints lock_entry jump_after
+  /\ ^prog_blop_ALL_DISTINCT_tm
+  /\ bir_get_current_statement ^prog c.bst_pc = SOME $ BSGen $ BStmtB $ BMCStmt_Assume e
+  ==> post_cond M c' lock_entry
+Proof
+  clstep_post_cond_inv_tac
+  (* BMCStmt_Assume *)
+  >> gvs[prog_bgcs,AND_IMP_INTRO,IMP_CONJ_THM,FORALL_AND_THM,prog_blop_ALL_DISTINCT]
+  >> qpat_assum `_ = c_bst_pc.bpc_label` $ assume_tac o GSYM
+  >> fs[]
+QED
+
+Theorem clstep_post_cond_inv_BStmt_Halt:
+  clstep (^prog) cid c M prom c'
+  /\ post_cond M c lock_entry
+  /\ well_formed cid M c
+  /\ wf_mem_vals M
+  /\ prog_individual_constraints lock_entry jump_after
+  /\ ^prog_blop_ALL_DISTINCT_tm
+  /\ bir_get_current_statement ^prog c.bst_pc = SOME $ BSGen $ BStmtE $ BStmt_Halt e
+  ==> post_cond M c' lock_entry
+Proof
+  clstep_post_cond_inv_tac
+  (* BStmt_Halt *)
+  >> gvs[prog_bgcs,AND_IMP_INTRO,IMP_CONJ_THM,FORALL_AND_THM,prog_blop_ALL_DISTINCT]
+  >> qpat_assum `_ = c_bst_pc.bpc_label` $ assume_tac o GSYM
+  >> fs[]
+QED
+
+Theorem clstep_post_cond_inv_BStmt_Jmp:
+  clstep (^prog) cid c M prom c'
+  /\ post_cond M c lock_entry
+  /\ well_formed cid M c
+  /\ wf_mem_vals M
+  /\ prog_individual_constraints lock_entry jump_after
+  /\ ^prog_blop_ALL_DISTINCT_tm
+  /\ bir_get_current_statement ^prog c.bst_pc = SOME $ BSGen $ BStmtE $ BStmt_Jmp e
+  ==> post_cond M c' lock_entry
+Proof
+  clstep_post_cond_inv_tac
+  (* BStmt_Jmp *)
+  >> fs[prog_blop_ALL_DISTINCT]
+  >> gvs[prog_bgcs]
+  >> fs[AND_IMP_INTRO,IMP_CONJ_THM,FORALL_AND_THM]
+  >> qpat_assum `_ = c_bst_pc.bpc_label` $ assume_tac o GSYM
+  >> fs[bir_envTheory.bir_var_name_def,bir_envTheory.bir_var_type_def,bir_read_reg_def,v_succ_def,v_fail_def]
+  >> rpt strip_tac
+  >> gs[bir_exec_stmt_jmp_eq,prog_blop,bir_block_pc_def,wordsTheory.dimword_64,bir_exec_stmt_jmp_bst_eq]
+  >> rpt $ goal_assum drule_all
+QED
+
+Theorem clstep_post_cond_inv_BSExt:
+  clstep (^prog) cid c M prom c'
+  /\ post_cond M c lock_entry
+  /\ well_formed cid M c
+  /\ wf_mem_vals M
+  /\ prog_individual_constraints lock_entry jump_after
+  /\ ^prog_blop_ALL_DISTINCT_tm
+  /\ bir_get_current_statement ^prog c.bst_pc = SOME $ BSExt R
+  ==> post_cond M c' lock_entry
+Proof
+  clstep_post_cond_inv_tac
+  (* We don't expect BSExt in programs *)
+  >> gvs[prog_bgcs]
+QED
+
+(* combination of previous theorems *)
+Theorem clstep_post_cond_inv:
+  clstep (^prog) cid c M prom c'
+  /\ post_cond M c lock_entry
+  /\ well_formed cid M c
+  /\ wf_mem_vals M
+  /\ prog_individual_constraints lock_entry jump_after
+  /\ ^prog_blop_ALL_DISTINCT_tm
+  ==> post_cond M c' lock_entry
+Proof
+  rpt strip_tac
+  >> imp_res_tac clstep_bgcs_imp
+  >> drule_then assume_tac bir_get_current_statement_SOME_MEM
+  >> drule_at (Pat `clstep`) clstep_preserves_wf
+  >> disch_then $ drule_at_then Any assume_tac
+  >> fs[prog_wf_ext]
+  >> imp_res_tac clstep_bgcs_cases
+  >> gvs[]
+  (* 12 subgoals *)
+  >~ [`BMCStmt_Load`]
+  >- (
+    drule_all clstep_post_cond_inv_BMCStmt_Load
+    >> fs[]
+  )
+  >~ [`BMCStmt_Store _ _ _ T _ _`]
+  >- (
+    drule clstep_post_cond_inv_BMCStmt_Store_fail
+    >> rpt $ disch_then $ drule_at Any
+    >> fs[]
+  )
+  >~ [`BMCStmt_Store`]
+  >- (
+    drule clstep_post_cond_inv_BMCStmt_Store
+    >> rpt $ disch_then $ drule_at Any
+    >> fs[]
+  )
+  >~ [`BMCStmt_Amo`]
+  >- (
+    drule clstep_post_cond_inv_BMCStmt_Amo
+    >> rpt $ disch_then $ drule_at Any
+    >> fs[]
+  )
+  >~ [`BMCStmt_Fence`]
+  >- (
+    drule clstep_post_cond_inv_BMCStmt_Fence
+    >> rpt $ disch_then $ drule_at Any
+    >> fs[]
+  )
+  >~ [`BStmt_CJmp`]
+  >- (
+    drule clstep_post_cond_inv_BMCStmt_CJmp
+    >> rpt $ disch_then $ drule_at Any
+    >> fs[]
+  )
+  >~ [`BMCStmt_Assign`]
+  >- (
+    drule clstep_post_cond_inv_BMCStmt_Assign
+    >> rpt $ disch_then $ drule_at Any
+    >> fs[]
+  )
+  >~ [`BMCStmt_Assert`]
+  >- (
+    drule clstep_post_cond_inv_BMCStmt_Assert
+    >> rpt $ disch_then $ drule_at Any
+    >> fs[]
+  )
+  >~ [`BMCStmt_Assume`]
+  >- (
+    drule clstep_post_cond_inv_BMCStmt_Assume
+    >> rpt $ disch_then $ drule_at Any
+    >> fs[]
+  )
+  >~ [`BStmt_Halt`]
+  >- (
+    drule clstep_post_cond_inv_BStmt_Halt
+    >> rpt $ disch_then $ drule_at Any
+    >> fs[]
+  )
+  >~ [`BStmt_Jmp`]
+  >- (
+    drule clstep_post_cond_inv_BStmt_Jmp
+    >> rpt $ disch_then $ drule_at Any
+    >> fs[]
+  )
+  >~ [`BSExt`]
+  >- (
+    drule clstep_post_cond_inv_BSExt
+    >> rpt $ disch_then $ drule_at Any
+    >> fs[]
+  )
+QED
 
 end
