src/theory/tools/promising/promising_thmsScript.sml
@@ -1,0 +1,853 @@
+(*
+ * Theorems about promising semantics
+ *)
+
+open HolKernel boolLib bossLib Parse;
+open listTheory rich_listTheory arithmeticTheory
+     wordsTheory bitstringTheory llistTheory wordsLib
+     finite_mapTheory string_numTheory relationTheory
+     bir_programTheory bir_promisingTheory
+     bir_promising_wfTheory bir_programLib;
+
+val _ = new_theory "promising_thms";
+
+(* TODO move closer to definition *)
+
+Theorem type_of_bir_imm_EQ_ELIMS:
+  !v0 v1.
+  type_of_bir_imm v0 = v1
+  <=> (?v. v0 = Imm1 v /\ v1 = Bit1)
+    \/ (?v. v0 = Imm8 v /\ v1 = Bit8)
+    \/ (?v. v0 = Imm16 v /\ v1 = Bit16)
+    \/ (?v. v0 = Imm32 v /\ v1 = Bit32)
+    \/ (?v. v0 = Imm64 v /\ v1 = Bit64)
+    \/ (?v. v0 = Imm128 v /\ v1 = Bit128)
+Proof
+  ntac 2 Cases
+  >> fs[bir_immTheory.type_of_bir_imm_def]
+QED
+
+(* clstep theorems *)
+
+Theorem clstep_bgcs_imp:
+  !p cid s M prom s'.
+    clstep p cid s M prom s'
+    ==> ?stmt. bir_get_current_statement p s.bst_pc = SOME stmt
+Proof
+  dsimp[clstep_cases]
+QED
+
+Theorem clstep_bgcs_cases:
+  !p cid c M prom c'.
+  clstep p cid c M prom c'
+  ==> ?stmt. bir_get_current_statement p c.bst_pc = SOME stmt /\ (
+    (?var a_e opt_cast xcl acq rel. stmt = BSGen $ BStmtB $ BMCStmt_Load var a_e opt_cast xcl acq rel)
+    \/ (?var_succ a_e v_e xcl acq rel. stmt = BSGen $ BStmtB $ BMCStmt_Store var_succ a_e v_e xcl acq rel /\ xcl /\ prom = [])
+    \/ (?var_succ a_e v_e xcl acq rel. stmt = BSGen $ BStmtB $ BMCStmt_Store var_succ a_e v_e xcl acq rel /\ ~(NULL prom))
+    \/ (?var a_e v_e acq rel. stmt = BSGen $ BStmtB $ BMCStmt_Amo var a_e v_e acq rel)
+    \/ (?K1 K2. stmt = BSGen $ BStmtB $ BMCStmt_Fence K1 K2)
+    \/ (?cond_e lbl1 lbl2. stmt = BSGen $ BStmtE $ BStmt_CJmp cond_e lbl1 lbl2)
+    \/ (?var e. stmt = BSGen $ BStmtB $ BMCStmt_Assign var e)
+    \/ (?e. stmt = BSGen $ BStmtB $ BMCStmt_Assert e)
+    \/ (?e. stmt = BSGen $ BStmtB $ BMCStmt_Assume e)
+    \/ (?e. stmt = BSGen $ BStmtE $ BStmt_Halt e)
+    \/ (?e. stmt = BSGen $ BStmtE $ BStmt_Jmp e)
+    \/ (?R. stmt = BSExt R))
+Proof
+  rpt strip_tac
+  >> gvs[clstep_cases,bmc_exec_general_stmt_exists]
+QED
+
+Theorem cstep_bgcs_imp:
+  !P prog cid s M prom s' M'.
+    cstep P prog cid s M prom s' M'
+    /\ M = M'
+    ==> ?stmt. bir_get_current_statement prog s.bst_pc = SOME stmt
+Proof
+  dsimp[clstep_cases,cstep_cases]
+QED
+
+
+Theorem bir_exec_stmt_cjmp_disj:
+  !p cond lbl1 lbl2 s.
+     (bir_exec_stmt_cjmp p cond (BLE_Label lbl1) (BLE_Label lbl2) s).bst_pc.bpc_label = s.bst_pc.bpc_label
+  \/ (bir_exec_stmt_cjmp p cond (BLE_Label lbl1) (BLE_Label lbl2) s).bst_pc.bpc_label = lbl1
+  \/ (bir_exec_stmt_cjmp p cond (BLE_Label lbl1) (BLE_Label lbl2) s).bst_pc.bpc_label = lbl2
+Proof
+  rw[bir_exec_stmt_cjmp_def,AllCaseEqs(),bir_state_set_typeerror_def,bir_exec_stmt_jmp_def,bir_exec_stmt_jmp_to_label_def,bir_block_pc_def,bir_eval_label_exp_def]
+  >> BasicProvers.every_case_tac
+  >> fs[]
+QED
+
+Theorem bir_exec_stmt_jmp_disj:
+  !p lbl s.
+  (bir_exec_stmt_jmp p (BLE_Label lbl) s).bst_pc.bpc_label = s.bst_pc.bpc_label
+  \/ ((bir_exec_stmt_jmp p (BLE_Label lbl) s).bst_pc.bpc_label = lbl
+    /\ (bir_exec_stmt_jmp p (BLE_Label lbl) s).bst_pc.bpc_index = 0)
+Proof
+  rw[bir_exec_stmt_jmp_def,bir_state_set_typeerror_def,bir_exec_stmt_jmp_to_label_def,bir_eval_label_exp_def,bir_block_pc_def]
+QED
+
+
+Theorem INDEX_FIND_append:
+  !ls n P ls'. INDEX_FIND n P (ls ++ ls') =
+  if EXISTS P ls then INDEX_FIND n P ls else INDEX_FIND (n + LENGTH ls) P ls'
+Proof
+  Induct >> rw[listTheory.INDEX_FIND_def] >> fs[arithmeticTheory.ADD1]
+QED
+
+Definition list_disj_def:
+  list_disj l1 l2 = !x. MEM x l1 ==> ~MEM x l2
+End
+
+Theorem list_disj_ALL_DISTINCT:
+  !l1 l2. ALL_DISTINCT (l1 ++ l2) ==> list_disj l1 l2
+Proof
+  rw[listTheory.ALL_DISTINCT_APPEND,list_disj_def]
+QED
+
+Theorem list_disj_nub:
+  list_disj (nub l1) l2 = list_disj l1 l2
+  /\ list_disj l2 (nub l1) = list_disj l2 l1
+Proof
+  fs[list_disj_def]
+QED
+
+Theorem list_disj_eq:
+  !l1 l2. list_disj l1 l2 = ALL_DISTINCT (nub l1 ++ nub l2)
+Proof
+  rw[listTheory.ALL_DISTINCT_APPEND,list_disj_def]
+QED
+
+Theorem list_disj_spec:
+  !l1 l2. list_disj l1 l2 =
+  !x. (MEM x l1 ==> ~MEM x l2) /\ (MEM x l2 ==> ~MEM x l1)
+Proof
+  rw[list_disj_def,EQ_IMP_THM]
+  >> PRED_ASSUM is_forall $ imp_res_tac o REWRITE_RULE[Once MONO_NOT_EQ]
+QED
+
+Theorem list_disj_spec_ho =
+  Ho_Rewrite.REWRITE_RULE[FORALL_AND_THM] list_disj_spec
+
+Theorem list_disj_sym:
+  !l1 l2. list_disj l1 l2 = list_disj l2 l1
+Proof
+  fs[list_disj_spec,AC CONJ_ASSOC CONJ_COMM]
+QED
+
+Theorem list_disj_sym_imp = iffLR list_disj_sym
+
+Theorem list_disj_append2:
+  !l1 l2 l3. list_disj l1 (l2 ++ l3) <=> list_disj l1 l2 /\ list_disj l1 l3
+Proof
+  dsimp[list_disj_def]
+QED
+
+Theorem list_disj_append1 =
+  ONCE_REWRITE_RULE[GSYM list_disj_sym] list_disj_append2;
+
+Theorem list_disj_sub:
+  list_disj l1 l2 /\ MEM a l1 ==> list_disj [a] l2
+Proof
+  fs[list_disj_def]
+QED
+
+Theorem list_disj_singleton:
+  list_disj [a] l1 = ~MEM a l1
+  /\ list_disj l1 [a] = ~MEM a l1
+Proof
+  fs[list_disj_def]
+QED
+
+Definition list_subset_def:
+  list_subset l1 l2 = !x. MEM x l1 ==> MEM x l2
+End
+
+Theorem list_subset_id:
+  !l1. list_subset l1 l1
+Proof
+  fs[list_subset_def]
+QED
+
+Theorem list_subset_trans:
+  !l1 l2 l3. list_subset l1 l2 /\ list_subset l2 l3
+  ==> list_subset l1 l3
+Proof
+  rw[list_subset_def]
+QED
+
+Theorem list_subset_EVERY:
+  !l1 l2. list_subset l1 l2 = EVERY (λx. MEM x l2) l1
+Proof
+  fs[listTheory.EVERY_MEM,list_subset_def]
+QED
+
+Theorem list_subset_append2_imp:
+  (!l1 l2 l3. list_subset l1 l3 ==> list_subset l1 (l2 ++ l3))
+  /\ !l1 l2 l3. list_subset l1 l2 ==> list_subset l1 (l2 ++ l3)
+Proof
+  simp[list_subset_def]
+QED
+
+Theorem bir_labels_of_program_APPEND:
+  !A B.
+    bir_labels_of_program (BirProgram $ A ++ B) =
+      bir_labels_of_program (BirProgram A)
+      ++ (bir_labels_of_program (BirProgram B))
+Proof
+  fs[bir_labels_of_program_def]
+QED
+
+Theorem bir_get_program_block_info_by_label_eq:
+  !p. set $ bir_labels_of_program p
+  = { l | ?i bl. bir_get_program_block_info_by_label p l = SOME (i,bl) }
+Proof
+  Cases >> rw[pred_setTheory.EXTENSION,bir_get_program_block_info_by_label_MEM]
+QED
+
+Theorem bir_get_program_block_info_by_label_APPEND_list_disj:
+  !A B label v.
+  bir_get_program_block_info_by_label (BirProgram A) label = SOME v
+  /\ list_disj (bir_labels_of_program $ BirProgram A)
+    (bir_labels_of_program $ BirProgram B)
+  ==>
+  bir_get_program_block_info_by_label (BirProgram (A ++ B)) label = SOME v
+Proof
+  fs[pairTheory.FORALL_PROD]
+  >> rw[bir_get_program_block_info_by_label_THM]
+  >> fs[rich_listTheory.EL_APPEND1]
+QED
+
+Theorem bir_get_program_block_info_by_label_APPEND2:
+  !A B label v.
+  bir_get_program_block_info_by_label (BirProgram A) label = NONE
+  ==>
+  bir_get_program_block_info_by_label (BirProgram (A ++ B)) label =
+    OPTION_MAP (λ(l,b). (l + LENGTH A,b)) $
+      bir_get_program_block_info_by_label (BirProgram B) label
+Proof
+  rw[bir_get_program_block_info_by_label_THM]
+  >> qmatch_goalsub_abbrev_tac `_ = x` >> Cases_on `x`
+  >> fs[bir_get_program_block_info_by_label_THM,pairTheory.LAMBDA_PROD,pairTheory.EXISTS_PROD]
+  >> dsimp[]
+  >> fs[bir_get_program_block_info_by_label_THM,listTheory.EL_APPEND_EQN]
+  >> rw[rich_listTheory.EL_MEM]
+QED
+
+Theorem bir_get_current_statement_SOME_MEM:
+  !prog pc x.
+  bir_get_current_statement prog pc = SOME x
+  ==> MEM pc.bpc_label $ bir_labels_of_program prog
+Proof
+  rw[bir_get_current_statement_def,AllCaseEqs(),bir_get_program_block_info_by_label_MEM]
+  >> fs[GSYM pairTheory.EXISTS_PROD]
+QED
+
+Theorem clstep_MEM_bir_labels_of_program:
+  !prog s s' M prom cid x.
+  clstep prog cid s M prom s'
+  ==> MEM s'.bst_pc.bpc_label $ bir_labels_of_program prog
+Proof
+  rw[clstep_cases,bir_state_read_view_updates_def,bir_get_current_statement_def,AllCaseEqs(),bir_get_program_block_info_by_label_MEM,bir_state_fulful_view_updates_def,fence_updates_def,bmc_exec_general_stmt_exists]
+  >> fs[bir_exec_stmt_jmp_to_label_mc_invar]
+  >> fs[bir_exec_stmt_cjmp_def,bir_exec_stmt_jmp_def,bir_exec_stmt_jmp_to_label_def,bir_exec_stmt_assert_def,bir_exec_stmt_assume_def,bir_exec_stmt_halt_def]
+  >> BasicProvers.every_case_tac
+  >> fs[bir_state_set_typeerror_def,bir_block_pc_def,bir_get_program_block_info_by_label_MEM]
+  >> gvs[bir_pc_next_def,GSYM pairTheory.EXISTS_PROD,pairTheory.ELIM_UNCURRY]
+QED
+
+Theorem bir_get_current_statement_MEM1:
+  !A B pc stmt.
+  bir_get_current_statement (BirProgram $ A ++ B) pc = SOME stmt
+  /\ MEM pc.bpc_label $ bir_labels_of_program $ BirProgram A
+  ==> bir_get_current_statement (BirProgram A) pc = SOME stmt
+Proof
+  fs[bir_get_current_statement_def,optionTheory.IS_SOME_EXISTS,bir_get_program_block_info_by_label_MEM]
+  >> rw[AllCaseEqs()]
+  >> qmatch_asmsub_rename_tac `bir_get_program_block_info_by_label (BirProgram $ A ++ B) _ = SOME x`
+  >> qmatch_asmsub_rename_tac `bir_get_program_block_info_by_label (BirProgram A) _ = SOME x'`
+  >> qsuff_tac `x = x'` >- (rw[] >> fs[])
+  >> PairCases_on `x` >> PairCases_on `x'`
+  >> Cases_on `x0 <> x'0`
+  >> gs[bir_get_program_block_info_by_label_THM,rich_listTheory.EL_APPEND1,arithmeticTheory.NOT_NUM_EQ,GSYM arithmeticTheory.LESS_EQ]
+  >> first_x_assum drule
+  >> gs[rich_listTheory.EL_APPEND1]
+QED
+
+Theorem bir_get_current_statement_MEM1':
+  !A B pc stmt.
+  bir_get_current_statement (BirProgram A) pc = SOME stmt
+  /\ list_disj (bir_labels_of_program $ BirProgram A)
+    (bir_labels_of_program $ BirProgram B)
+  ==> bir_get_current_statement (BirProgram $ A ++ B) pc = SOME stmt
+Proof
+  rpt strip_tac
+  >> imp_res_tac bir_get_current_statement_SOME_MEM
+  >> fs[bir_get_current_statement_def,optionTheory.IS_SOME_EXISTS,bir_get_program_block_info_by_label_MEM]
+  >> drule_all_then assume_tac bir_get_program_block_info_by_label_APPEND_list_disj
+  >> fs[AllCaseEqs(),pairTheory.ELIM_UNCURRY,PULL_EXISTS]
+QED
+
+Theorem bir_get_current_statement_BirProgram_APPEND:
+  !A B pc.
+  list_disj (bir_labels_of_program $ BirProgram A)
+    (bir_labels_of_program $ BirProgram B)
+  ==>
+    bir_get_current_statement (BirProgram $ A ++ B) pc =
+      if IS_SOME $ bir_get_program_block_info_by_label (BirProgram A) pc.bpc_label
+      then bir_get_current_statement (BirProgram A) pc
+      else bir_get_current_statement (BirProgram B) pc
+Proof
+  rw[bir_get_current_statement_def,optionTheory.IS_SOME_EXISTS]
+  >- (
+    drule_all_then assume_tac bir_get_program_block_info_by_label_APPEND_list_disj
+    >> fs[]
+  )
+  >> qmatch_asmsub_abbrev_tac `~?x. blah = SOME x` >> Cases_on `blah`
+  >> fs[bir_get_program_block_info_by_label_APPEND2]
+  >> qmatch_goalsub_abbrev_tac `OPTION_MAP _ bgpbibl` >> Cases_on `bgpbibl`
+  >> fs[]
+  >> qmatch_asmsub_rename_tac `SOME x` >> PairCases_on `x`
+  >> fs[]
+QED
+
+Theorem bir_get_current_statement_MEM2:
+  !A B pc stmt.
+  bir_get_current_statement (BirProgram $ A ++ B) pc = SOME stmt
+  /\ list_disj (bir_labels_of_program $ BirProgram A)
+      (bir_labels_of_program $ BirProgram B)
+  /\ MEM pc.bpc_label $ bir_labels_of_program $ BirProgram B
+  ==> bir_get_current_statement (BirProgram B) pc = SOME stmt
+Proof
+  rpt strip_tac
+  >> drule_then assume_tac bir_get_current_statement_BirProgram_APPEND
+  >> fs[optionTheory.IS_SOME_EXISTS,Once list_disj_sym,list_disj_def]
+  >> first_x_assum $ drule_then assume_tac
+  >> fs[bir_get_program_block_info_by_label_MEM,GSYM pairTheory.FORALL_PROD]
+QED
+
+Theorem bir_get_current_statement_APPEND1:
+  !A B pc.
+  list_disj (bir_labels_of_program $ BirProgram A)
+      (bir_labels_of_program $ BirProgram B)
+  /\ MEM pc.bpc_label $ bir_labels_of_program $ BirProgram A
+  ==>
+    bir_get_current_statement (BirProgram $ A ++ B) pc =
+      bir_get_current_statement (BirProgram A) pc
+Proof
+  rpt strip_tac
+  >> fs[bir_get_current_statement_BirProgram_APPEND,list_disj_def]
+  >> first_x_assum $ drule_then assume_tac
+  >> fs[AllCaseEqs(),bir_get_program_block_info_by_label_eq]
+QED
+
+Theorem bir_get_current_statement_APPEND2:
+  !A B pc.
+  list_disj (bir_labels_of_program $ BirProgram A)
+      (bir_labels_of_program $ BirProgram B)
+  /\ MEM pc.bpc_label $ bir_labels_of_program $ BirProgram B
+  ==>
+    bir_get_current_statement (BirProgram $ A ++ B) pc =
+      bir_get_current_statement (BirProgram B) pc
+Proof
+  rpt strip_tac
+  >> fs[bir_get_current_statement_BirProgram_APPEND,Once list_disj_sym,list_disj_def]
+  >> first_x_assum $ drule_then assume_tac
+  >> fs[AllCaseEqs(),bir_get_program_block_info_by_label_eq,GSYM pairTheory.FORALL_PROD]
+  >> Cases_on `bir_get_program_block_info_by_label (BirProgram A) pc.bpc_label`
+  >> fs[]
+QED
+
+Theorem bir_get_program_block_info_by_label_IS_NONE_NOT_MEM:
+  !A lbl. IS_NONE $ bir_get_program_block_info_by_label (BirProgram A) lbl
+  ==> ~(MEM lbl $ bir_labels_of_program $ BirProgram A)
+Proof
+  fs[bir_get_program_block_info_by_label_MEM,GSYM pairTheory.EXISTS_PROD,optionTheory.IS_SOME_EXISTS]
+QED
+
+Theorem bir_get_program_block_info_by_label_IS_SOME_MEM:
+  !A lbl. IS_SOME $ bir_get_program_block_info_by_label (BirProgram A) lbl
+  ==> MEM lbl $ bir_labels_of_program $ BirProgram A
+Proof
+  fs[bir_get_program_block_info_by_label_MEM,GSYM pairTheory.EXISTS_PROD,optionTheory.IS_SOME_EXISTS]
+QED
+
+Theorem bir_get_current_statement_APPEND_cases:
+  !A B pc.
+  list_disj (bir_labels_of_program $ BirProgram A)
+      (bir_labels_of_program $ BirProgram B)
+  ==>
+    (~(MEM pc.bpc_label $ bir_labels_of_program $ BirProgram A)
+    /\ bir_get_current_statement (BirProgram $ A ++ B) pc =
+      bir_get_current_statement (BirProgram B) pc)
+    \/ (MEM pc.bpc_label $ bir_labels_of_program $ BirProgram A
+    /\ ~(MEM pc.bpc_label $ bir_labels_of_program $ BirProgram B)
+    /\ bir_get_current_statement (BirProgram $ A ++ B) pc =
+      bir_get_current_statement (BirProgram A) pc)
+Proof
+  rw[bir_get_current_statement_BirProgram_APPEND,iffLR list_disj_sym]
+  >> fs[bir_get_program_block_info_by_label_IS_NONE_NOT_MEM,bir_get_program_block_info_by_label_IS_SOME_MEM,list_disj_sym_imp,list_disj_def]
+QED
+
+Theorem bir_get_current_statement_APPEND3_cases:
+  !A B C pc.
+  list_disj (bir_labels_of_program $ BirProgram A)
+      (bir_labels_of_program $ BirProgram B)
+  /\ list_disj (bir_labels_of_program $ BirProgram A)
+      (bir_labels_of_program $ BirProgram C)
+  /\ list_disj (bir_labels_of_program $ BirProgram B)
+      (bir_labels_of_program $ BirProgram C)
+  ==>
+    (MEM pc.bpc_label $ bir_labels_of_program $ BirProgram A
+      /\ ~(MEM pc.bpc_label $ bir_labels_of_program $ BirProgram B)
+      /\ ~(MEM pc.bpc_label $ bir_labels_of_program $ BirProgram C)
+      /\ bir_get_current_statement (BirProgram $ A ++ B ++ C) pc =
+        bir_get_current_statement (BirProgram A) pc)
+    \/ (~(MEM pc.bpc_label $ bir_labels_of_program $ BirProgram A)
+      /\ MEM pc.bpc_label $ bir_labels_of_program $ BirProgram B
+      /\ ~(MEM pc.bpc_label $ bir_labels_of_program $ BirProgram C)
+      /\ bir_get_current_statement (BirProgram $ A ++ B ++ C) pc =
+        bir_get_current_statement (BirProgram B) pc)
+    \/ (~(MEM pc.bpc_label $ bir_labels_of_program $ BirProgram A)
+      /\ ~(MEM pc.bpc_label $ bir_labels_of_program $ BirProgram B)
+      /\ bir_get_current_statement (BirProgram $ A ++ B ++ C) pc =
+        bir_get_current_statement (BirProgram C) pc)
+Proof
+  rpt strip_tac
+  >> qspecl_then [`A`,`B ++ C`,`pc`] assume_tac bir_get_current_statement_APPEND_cases
+  >> qspecl_then [`B`,`C`,`pc`] assume_tac bir_get_current_statement_APPEND_cases
+  >> gs[list_disj_sym_imp,bir_labels_of_program_APPEND,list_disj_append1,list_disj_append2]
+QED
+
+Theorem bir_get_current_statement_three:
+  !pc A B C.
+  MEM pc.bpc_label $ bir_labels_of_program $ BirProgram $ A ++ B ++ C
+  /\ list_disj (bir_labels_of_program $ BirProgram A)
+    (bir_labels_of_program $ BirProgram B)
+  /\ list_disj (bir_labels_of_program $ BirProgram B)
+    (bir_labels_of_program $ BirProgram C)
+  /\ list_disj (bir_labels_of_program $ BirProgram A)
+    (bir_labels_of_program $ BirProgram C)
+  /\ ~(MEM pc.bpc_label $ bir_labels_of_program $ BirProgram B)
+  ==>
+  (MEM pc.bpc_label $ bir_labels_of_program $ BirProgram A
+  /\ ~(MEM pc.bpc_label $ bir_labels_of_program $ BirProgram C)
+  /\ bir_get_current_statement (BirProgram $ A ++ B ++ C) pc = bir_get_current_statement (BirProgram $ A) pc)
+  \/
+  (~(MEM pc.bpc_label $ bir_labels_of_program $ BirProgram A)
+  /\ MEM pc.bpc_label $ bir_labels_of_program $ BirProgram C
+  /\ bir_get_current_statement (BirProgram $ A ++ B ++ C) pc = bir_get_current_statement (BirProgram $ C) pc)
+Proof
+  rpt strip_tac
+  >> qmatch_goalsub_abbrev_tac `(P /\ ~Q /\ _) \/ (~P /\ Q /\ _)`
+  >> Cases_on `P`
+  >> gs[list_disj_sym_imp,bir_get_current_statement_APPEND1,list_disj_append1,list_disj_append2,bir_get_current_statement_APPEND2,bir_labels_of_program_APPEND]
+  >> gs[list_disj_spec_ho]
+QED
+
+Theorem well_formed_mem_read_view_zero:
+  !cid M s l.
+  well_formed cid M s ==> mem_read_view (s.bst_fwdb l) 0 = 0
+Proof
+  rw[mem_read_view_def,well_formed_fwdb_def,well_formed_def]
+  >> qmatch_asmsub_rename_tac `s.bst_fwdb l`
+  >> first_x_assum $ qspec_then `l` assume_tac
+  >> fs[]
+QED
+
+(* properties of permutation of program instructions *)
+
+Theorem bir_labels_of_program_PERM:
+  !p p'. PERM p p'
+  ==> PERM (bir_labels_of_program (BirProgram p))
+    (bir_labels_of_program (BirProgram p'))
+Proof
+  ho_match_mp_tac sortingTheory.PERM_lifts_monotonicities
+  >> fs[bir_labels_of_program_APPEND]
+  >> rpt strip_tac
+  >> irule_at Any EQ_REFL
+  >> fs[]
+QED
+
+Theorem bir_labels_of_program_ALL_DISTINCT:
+  !p p'. PERM p p'
+  ==> ALL_DISTINCT (bir_labels_of_program (BirProgram p))
+    = ALL_DISTINCT (bir_labels_of_program (BirProgram p'))
+Proof
+  fs[bir_labels_of_program_PERM,sortingTheory.ALL_DISTINCT_PERM]
+QED
+
+Theorem PERMUTES_count_less:
+  k < n /\ f PERMUTES count n ==> f k < n
+Proof
+  fs[pred_setTheory.BIJ_ALT,pred_setTheory.FUNSET]
+QED
+
+Theorem INDEX_FIND_ALL_DISTINCT:
+  !f p p' z0 z1 a. PERM p p'
+  /\ ALL_DISTINCT (MAP f p)
+  /\ ALL_DISTINCT (MAP f p')
+  /\ INDEX_FIND 0 (λx. f x = a) p = SOME (z0,z1)
+  ==> ?z'. INDEX_FIND 0 (λx. f x = a) p' = SOME z' /\ SND z' = z1
+Proof
+  rpt strip_tac
+  >> fs[bir_auxiliaryTheory.INDEX_FIND_EQ_SOME_0,pairTheory.EXISTS_PROD,sortingTheory.PERM_BIJ_IFF,LENGTH_GENLIST]
+  >> qmatch_asmsub_rename_tac `n < LENGTH p`
+  >> cheat (* properties about BIJ functions (PERMUTES) *)
+QED
+
+Theorem bir_get_program_block_info_by_label_PERM:
+  PERM p p' /\ ALL_DISTINCT $ bir_labels_of_program $ BirProgram p
+  ==> OPTION_MAP SND $ bir_get_program_block_info_by_label (BirProgram p) label =
+      OPTION_MAP SND $ bir_get_program_block_info_by_label (BirProgram p') label
+Proof
+  rpt strip_tac
+  >> qmatch_goalsub_abbrev_tac`OPTION_MAP SND a = OPTION_MAP SND b`
+  >> drule_all_then assume_tac $ iffLR bir_labels_of_program_ALL_DISTINCT
+  >> fs[bir_get_program_block_info_by_label_def]
+  >> Cases_on `a`
+  >> fs[markerTheory.Abbrev_def,bir_auxiliaryTheory.INDEX_FIND_EQ_NONE]
+  >- (
+    drule_then irule $ iffLR sortingTheory.PERM_EVERY
+    >> fs[]
+  )
+  >> qmatch_asmsub_rename_tac `SOME x` >> PairCases_on `x`
+  >> fs[pairTheory.EXISTS_PROD,bir_labels_of_program_def]
+  >> qpat_x_assum `SOME _ = _` $ assume_tac o GSYM
+  >> qmatch_asmsub_abbrev_tac `MAP f`
+  >> rpt $ pop_assum mp_tac
+  >> CONV_TAC $ DEPTH_CONV ETA_CONV
+  >> rpt $ disch_then strip_assume_tac
+  >> qspec_then `f` mp_tac INDEX_FIND_ALL_DISTINCT
+  >> rpt $ disch_then drule
+  >> unabbrev_all_tac
+  >> fs[]
+  >> disch_then $ drule_then assume_tac
+  >> fs[pairTheory.EXISTS_PROD]
+QED
+
+Theorem bir_get_current_statement_PERM:
+  !p p' pc.
+  PERM p p' /\ ALL_DISTINCT $ bir_labels_of_program $ BirProgram p
+  ==> bir_get_current_statement (BirProgram p) pc =
+      bir_get_current_statement (BirProgram p') pc
+Proof
+  rpt strip_tac
+  >> drule_all bir_get_program_block_info_by_label_PERM
+  >> dsimp[bir_get_current_statement_def,optionTheory.option_case_compute,AllCaseEqs()]
+  >> rw[DISJ_EQ_IMP]
+  >> ntac 2 (pairarg_tac >> gvs[])
+  >- (
+    qmatch_asmsub_abbrev_tac `IS_SOME a ==> _`
+    >> Cases_on `a` >> gvs[markerTheory.Abbrev_def]
+    >> qmatch_asmsub_rename_tac `bir_get_program_block_info_by_label _ pc.bpc_label`
+    >> qpat_x_assum `SOME _ = _` $ assume_tac o GSYM
+    >> first_x_assum $ qspec_then `pc.bpc_label` assume_tac
+    >> gvs[]
+  )
+  >> gvs[optionTheory.IS_SOME_EXISTS]
+  >> qmatch_asmsub_rename_tac `bir_get_program_block_info_by_label _ pc.bpc_label`
+  >> first_x_assum $ qspec_then `pc.bpc_label` assume_tac
+  >> gvs[]
+QED
+
+Theorem bir_exec_stmt_jmp_to_label_PERM:
+  !p p' lbl c.
+  PERM p p' /\ ALL_DISTINCT $ bir_labels_of_program $ BirProgram p
+  ==> bir_exec_stmt_jmp_to_label (BirProgram p) lbl c
+    = bir_exec_stmt_jmp_to_label (BirProgram p') lbl c
+Proof
+  dsimp[bir_exec_stmt_jmp_to_label_def,optionTheory.option_case_compute,COND_RAND,COND_RATOR,COND_EXPAND_OR]
+  >> rpt strip_tac
+  >> drule_then assume_tac bir_labels_of_program_PERM
+  >> dxrule_then assume_tac PERM_MEM
+  >> csimp[]
+QED
+
+Theorem bir_exec_stmt_jmp_PERM:
+  PERM p p' /\ ALL_DISTINCT $ bir_labels_of_program $ BirProgram p
+  ==> bir_exec_stmt_jmp (BirProgram p) lbl c
+    = bir_exec_stmt_jmp (BirProgram p') lbl c
+Proof
+  dsimp[bir_exec_stmt_jmp_def,optionTheory.option_case_compute,COND_RAND]
+  >> rpt strip_tac
+  >> fs[bir_exec_stmt_jmp_to_label_PERM]
+QED
+
+Theorem bir_exec_stmt_cjmp_PERM:
+  PERM p p' /\ ALL_DISTINCT $ bir_labels_of_program $ BirProgram p
+  ==> bir_exec_stmt_cjmp (BirProgram p) cond_e lbl1 lbl2 c
+    = bir_exec_stmt_cjmp (BirProgram p') cond_e lbl1 lbl2 c
+Proof
+  rpt strip_tac
+  >> dsimp[bir_exec_stmt_cjmp_def,optionTheory.option_case_compute,COND_RAND,COND_EXPAND_OR]
+  >> csimp[bir_exec_stmt_jmp_PERM]
+  >> qmatch_goalsub_abbrev_tac `IS_SOME a /\ IS_SOME b`
+  >> Cases_on `a` >> Cases_on `b` >> fs[]
+QED
+
+Theorem clstep_permute_prog:
+  !p p' cid c M prom c'.
+  PERM p p' /\ ALL_DISTINCT $ bir_labels_of_program $ BirProgram p
+  ==>
+  clstep (BirProgram p) cid c M prom c' = clstep (BirProgram p') cid c M prom c'
+Proof
+  dsimp[EQ_IMP_THM]
+  >> conj_asm2_tac
+  >- (
+    rpt strip_tac
+    >> first_x_assum irule
+    >> fs[PULL_EXISTS]
+    >> drule_then (irule_at Any) $ iffLR sortingTheory.PERM_SYM
+    >> dxrule bir_labels_of_program_ALL_DISTINCT
+    >> fs[]
+  )
+  >> rpt strip_tac
+  >> drule_then strip_assume_tac clstep_bgcs_imp
+  >> drule_then assume_tac bir_labels_of_program_ALL_DISTINCT
+  >> qmatch_asmsub_abbrev_tac `bir_get_current_statement _ c.bst_pc`
+  >> drule_all_then (qspec_then `c.bst_pc` assume_tac) bir_get_current_statement_PERM
+  >> gvs[clstep_cases,bmc_exec_general_stmt_exists]
+  >> dsimp[]
+  >> gvs[bir_exec_stmt_jmp_PERM]
+  >~ [`BMCStmt_Load`]
+  >- (
+    qpat_assum `mem_read _ _ _ = _` $ irule_at Any
+    >> rpt $ goal_assum drule
+    >> fs[]
+  )
+  >~ [`BMCStmt_Store`]
+  >- rpt (rpt $ goal_assum drule >> fs[])
+  >~ [`BMCStmt_Amo`]
+  >- rpt (rpt $ goal_assum drule >> fs[])
+  >~ [`BStmt_CJmp`]
+  >- (
+    goal_assum drule
+    >> drule_all bir_exec_stmt_cjmp_PERM
+    >> fs[]
+  )
+  >~ [`BMCStmt_Assign`]
+  >- (
+    rpt $ goal_assum drule
+    >> fs[]
+  )
+  >~ [`BMCStmt_Store`]
+  >- rpt (rpt $ goal_assum drule >> fs[])
+  >~ [`BSExt`]
+  >- (
+    drule_then assume_tac bir_labels_of_program_PERM
+    >> dxrule_all $ iffRL PERM_MEM
+    >> fs[]
+  )
+QED
+
+(* read a variable from a state *)
+
+Definition bir_read_reg_def:
+  bir_read_reg var env v <=>
+    bir_eval_exp (BExp_Den $ BVar var $ BType_Imm Bit64) env
+    = SOME $ BVal_Imm $ Imm64 v
+End
+
+Theorem bir_read_reg_prime =
+  bir_read_reg_def
+  |> CONV_RULE $ ONCE_DEPTH_CONV $ (RHS_CONV o ONCE_REWRITE_CONV o single) EQ_SYM_EQ
+  |> GSYM
+
+Theorem bir_read_reg_update:
+  !f var v. bir_read_reg var (BEnv f(|var |-> SOME $ BVal_Imm $ Imm64 v|)) v
+Proof
+  rw[bir_read_reg_def,bir_expTheory.bir_eval_exp_def,bir_envTheory.bir_env_read_def,bir_envTheory.bir_env_check_type_def,bir_envTheory.bir_env_lookup_type_def,bir_envTheory.bir_var_type_def,bir_envTheory.bir_var_name_def,bir_envTheory.bir_env_lookup_def,combinTheory.APPLY_UPDATE_THM,bir_valuesTheory.type_of_bir_val_def,bir_immTheory.type_of_bir_imm_def]
+QED
+
+Theorem bir_env_lookup_update:
+  !var v f.
+  bir_env_lookup var (BEnv f(|var |-> SOME $ BVal_Imm $ Imm64 v|))
+  = SOME $ BVal_Imm $ Imm64 v
+Proof
+  rw[bir_expTheory.bir_eval_exp_def,bir_envTheory.bir_env_read_def,bir_envTheory.bir_env_check_type_def,bir_envTheory.bir_env_lookup_type_def,bir_envTheory.bir_var_type_def,bir_envTheory.bir_var_name_def,bir_envTheory.bir_env_lookup_def,combinTheory.APPLY_UPDATE_THM,bir_valuesTheory.type_of_bir_val_def,bir_immTheory.type_of_bir_imm_def]
+QED
+
+Theorem bir_read_reg_env_update_cast64:
+  !env var new_env v.
+  env_update_cast64 var (BVal_Imm $ Imm64 v) (BType_Imm Bit64) env = SOME new_env
+  ==> bir_read_reg var new_env v
+Proof
+  Cases >> EVAL_TAC
+  >> rw[env_update_cast64_def,bir_envTheory.bir_env_update_def,bir_read_reg_def]
+  >> fs[bir_env_lookup_update,bir_valuesTheory.type_of_bir_val_EQ_ELIMS,type_of_bir_imm_EQ_ELIMS]
+QED
+
+Definition bir_read_reg_zero_def:
+  bir_read_reg_zero var env = bir_read_reg var env 0w
+End
+
+Theorem bir_read_reg_imp:
+  !f var v.
+  f var = SOME (BVal_Imm (Imm64 v)) ==> bir_read_reg var (BEnv f) v
+Proof
+  rw[bir_read_reg_zero_def,bir_read_reg_def,bir_expTheory.bir_eval_exp_def,bir_envTheory.bir_env_check_type_def,bir_envTheory.bir_var_type_def,bir_envTheory.bir_var_name_def,bir_envTheory.bir_env_lookup_def,bir_envTheory.bir_env_lookup_type_def,bir_envTheory.bir_env_read_def,type_of_bir_imm_EQ_ELIMS,bir_valuesTheory.type_of_bir_val_EQ_ELIMS]
+QED
+
+Definition bir_read_reg_nonzero_def:
+  bir_read_reg_nonzero var env = ?v. bir_read_reg var env v /\ v <> 0w
+End
+
+
+
+Theorem mem_get_EVERY:
+  !t M l v f. mem_get M l t = SOME v /\ 0 < t /\ EVERY f M ==> f v
+Proof
+  Cases >> rw[CaseEq"option"]
+  >> gvs[mem_get_def,CaseEq"option",listTheory.oEL_THM,listTheory.EVERY_EL]
+QED
+
+Definition wf_mem_val_def:
+  wf_mem_val (m : mem_msg_t) = ?v'. m.val = BVal_Imm $ Imm64 v'
+End
+
+Definition wf_mem_vals_def:
+  wf_mem_vals M = EVERY wf_mem_val M
+End
+
+Theorem wf_mem_vals_mem_read:
+  !t M l v. mem_read M l t = SOME v /\ wf_mem_vals M
+  ==> ?v'. v = BVal_Imm $ Imm64 v'
+Proof
+  Cases >> rpt strip_tac
+  >> fs[mem_read_zero,mem_read_def,CaseEq"option",wf_mem_vals_def]
+  >> drule_then (dxrule_at Any) mem_get_EVERY
+  >> fs[wf_mem_val_def]
+QED
+
+Definition wf_mem_loc_def:
+  wf_mem_loc (m :mem_msg_t) = ?v'. m.loc = BVal_Imm $ Imm64 v'
+End
+
+Definition wf_mem_locs_def:
+  wf_mem_locs M = EVERY wf_mem_loc M
+End
+
+Theorem wf_mem_locs_mem_get:
+  !t M l v f. mem_get M l t = SOME v /\ 0 < t /\ wf_mem_locs M
+  ==> wf_mem_loc v
+Proof
+  rw[wf_mem_locs_def]
+  >> drule_all_then irule mem_get_EVERY
+QED
+
+Theorem xclfail_update_env_SOME:
+  !env name new_env.
+  xclfail_update_env (BVar name (BType_Imm Bit64)) env = SOME new_env
+  <=> ?f. env = BEnv f /\ f name <> NONE
+    /\ new_env = BEnv f(|name |-> SOME $ BVal_Imm v_fail |)
+Proof
+  Cases >> rpt gen_tac
+  >> CONV_TAC $ LAND_CONV EVAL
+  >> fs[EQ_IMP_THM,v_fail_def]
+QED
+
+Theorem bir_env_update_SOME_eq =
+  EVAL o Term $ `bir_env_update var (BVal_Imm v) (BType_Imm ty) (BEnv f) = SOME new_env`
+ |> SIMP_RULE std_ss [COND_RATOR,COND_RAND,bir_valuesTheory.type_of_bir_val_EQ_ELIMS,type_of_bir_imm_EQ_ELIMS]
+ |> GEN_ALL
+
+Theorem bir_env_update_SOME_eq' =
+  CONV_RULE (ONCE_DEPTH_CONV $ LAND_CONV $ ONCE_REWRITE_CONV[EQ_SYM_EQ]) bir_env_update_SOME_eq
+
+Theorem bir_eval_exp_BExp_Den_update_eq:
+  !name v f. bir_eval_exp (BExp_Den (BVar name (BType_Imm Bit64)))
+    (BEnv f(|name |-> SOME (BVal_Imm (Imm64 v ))|)) =
+      SOME (BVal_Imm (Imm64 v))
+Proof
+  fs[bir_expTheory.bir_eval_exp_def,bir_envTheory.bir_env_check_type_def,bir_envTheory.bir_var_type_def,bir_envTheory.bir_var_name_def,bir_envTheory.bir_env_lookup_def,bir_envTheory.bir_env_lookup_type_def,bir_envTheory.bir_env_read_def,PULL_EXISTS,bir_valuesTheory.type_of_bir_val_EQ_ELIMS,type_of_bir_imm_EQ_ELIMS,combinTheory.APPLY_UPDATE_THM]
+QED
+
+Theorem bir_eval_exp_BExp_Den_update_eq':
+  !name name' v f.
+    name <> name' ==>
+    bir_eval_exp (BExp_Den (BVar name (BType_Imm Bit64)))
+      (BEnv f(|name' |-> SOME v|)) =
+    bir_eval_exp (BExp_Den (BVar name (BType_Imm Bit64))) (BEnv f)
+Proof
+  fs[bir_expTheory.bir_eval_exp_def,bir_envTheory.bir_env_read_def,bir_envTheory.bir_env_check_type_def,bir_envTheory.bir_var_type_def,bir_envTheory.bir_var_name_def,bir_envTheory.bir_env_lookup_def,bir_envTheory.bir_env_lookup_type_def,bir_valuesTheory.type_of_bir_val_EQ_ELIMS,type_of_bir_imm_EQ_ELIMS,combinTheory.APPLY_UPDATE_THM]
+QED
+
+Theorem fulfil_update_env_BVar_eq:
+  !env new_env name.
+  fulfil_update_env (BVar name (BType_Imm Bit64)) T env = SOME new_env
+  <=> ?f. env = BEnv f /\ f name <> NONE
+    /\ new_env = BEnv f(|name |-> SOME $ BVal_Imm v_succ |)
+Proof
+  Cases >> rpt gen_tac
+  >> CONV_TAC $ LAND_CONV EVAL
+  >> fs[EQ_IMP_THM,v_succ_def]
+QED
+
+Theorem bir_dest_bool_val_false =
+  EVAL ``bir_dest_bool_val $ BVal_Imm $ Imm1 0w``
+
+Theorem bir_dest_bool_val_true =
+  EVAL ``bir_dest_bool_val $ BVal_Imm $ Imm1 $ -1w``
+
+Theorem bir_dest_bool_val_true' =
+  EVAL ``bir_dest_bool_val $ BVal_Imm $ Imm1 1w``
+
+Theorem bir_read_reg_bir_env_read:
+  bir_env_read (BVar var (BType_Imm Bit64)) env = SOME (BVal_Imm (Imm64 v))
+  <=> bir_read_reg var env v
+Proof
+  fs[bir_read_reg_def,bir_envTheory.bir_env_read_def,bir_expTheory.bir_eval_exp_def,bir_envTheory.bir_var_type_def,bir_envTheory.bir_var_name_def]
+QED
+
+(* TODO generalise *)
+Theorem bir_eval_exp_BExp_UnaryExp:
+  bir_read_reg var env x
+  ==> bir_eval_exp (BExp_UnaryExp BIExp_Not (BExp_BinPred BIExp_Equal
+                (BExp_Den (BVar var (BType_Imm Bit64)))
+                (BExp_Const (Imm64 v)))) env
+                = SOME $ BVal_Imm $ Imm1 (if x = v then 0w else 1w)
+Proof
+  fs[bir_expTheory.bir_eval_exp_def,bir_expTheory.bir_eval_unary_exp_def,bir_expTheory.bir_eval_unary_exp_def,bir_expTheory.bir_eval_bin_pred_REWRS,type_of_bir_imm_EQ_ELIMS,bir_exp_immTheory.bir_bin_pred_def,bir_exp_immTheory.bir_bin_pred_GET_OPER_def,GSYM bir_read_reg_bir_env_read]
+  >> fs[bir_immTheory.bool2b_def,bir_exp_immTheory.bir_unary_exp_def,bir_exp_immTheory.bir_unary_exp_GET_OPER_def]
+  >> strip_tac
+  >> EVAL_TAC
+  >> fs[COND_RAND,bir_auxiliaryTheory.word1_neg]
+QED
+
+Theorem bir_eval_exp_BExp_UnaryExp':
+  bir_read_reg var env x
+  ==> (bir_eval_exp (BExp_UnaryExp BIExp_Not (BExp_BinPred BIExp_Equal
+                (BExp_Den (BVar var (BType_Imm Bit64)))
+                (BExp_Const (Imm64 v)))) env
+                = SOME w
+        <=> w = BVal_Imm $ Imm1 (if x = v then 0w else 1w))
+Proof
+  fs[bir_expTheory.bir_eval_exp_def,bir_expTheory.bir_eval_unary_exp_def,bir_expTheory.bir_eval_unary_exp_def,bir_expTheory.bir_eval_bin_pred_REWRS,type_of_bir_imm_EQ_ELIMS,bir_exp_immTheory.bir_bin_pred_def,bir_exp_immTheory.bir_bin_pred_GET_OPER_def,GSYM bir_read_reg_bir_env_read]
+  >> fs[bir_immTheory.bool2b_def,bir_exp_immTheory.bir_unary_exp_def,bir_exp_immTheory.bir_unary_exp_GET_OPER_def]
+  >> strip_tac
+  >> EVAL_TAC
+  >> fs[COND_RAND,bir_auxiliaryTheory.word1_neg]
+QED
+
+Theorem bir_eval_exp_SOME:
+  !exp env v. bir_eval_exp exp env = SOME v
+  <=> ?f. bir_eval_exp exp (BEnv f) = SOME v /\ env = BEnv f
+Proof
+  Cases_on `env` >> fs[]
+QED
+
+Theorem bir_eval_exp_SOME' =
+  CONV_RULE (ONCE_DEPTH_CONV $ LAND_CONV $ ONCE_REWRITE_CONV[EQ_SYM_EQ]) 
+  bir_eval_exp_SOME
+
+Theorem bir_exec_stmt_jmp_eq:
+  MEM (BL_Address x) $ bir_labels_of_program prog
+  ==> (bir_exec_stmt_jmp prog (BLE_Label $ BL_Address x) s).bst_pc =
+    bir_block_pc $ BL_Address x
+Proof
+  fs[bir_exec_stmt_jmp_def,bir_eval_label_exp_def,bir_exec_stmt_jmp_to_label_def]
+QED
+
+val _ = export_theory ();
